disk-betree/BetreeBlockCacheSystem.dfy
@@ -1,0 +1,131 @@
+include "Disk.dfy"
+include "BlockCache.dfy"
+include "../lib/Maps.dfy"
+include "../lib/sequences.dfy"
+include "BlockCacheSystem.dfy"
+include "BetreeBlockCache.dfy"
+
+module BetreeGraphBlockCacheSystem refines BlockCacheSystem {
+  import M = BetreeGraphBlockCache
+}
+
+module BetreeBlockCacheSystem {
+  import opened Maps
+  import opened Sequences
+
+  import BC = BetreeGraphBlockCache
+  import BCS = BetreeGraphBlockCacheSystem
+  import DB = DiskBetree
+  import M = BetreeBlockCache
+  import D = Disk
+
+  type Constants = BCS.Constants
+  type Variables = BCS.Variables
+  type DiskOp = M.DiskOp
+
+  predicate Init(k: Constants, s: Variables)
+  {
+    BCS.Init(k, s)
+  }
+
+  datatype Step =
+    | MachineStep(dop: DiskOp)
+    | CrashStep
+
+  predicate Machine(k: Constants, s: Variables, s': Variables, dop: DiskOp)
+  {
+    && M.Next(k.machine, s.machine, s'.machine, dop)
+    && D.Next(k.disk, s.disk, s'.disk, dop)
+  }
+
+  predicate Crash(k: Constants, s: Variables, s': Variables)
+  {
+    && M.Init(k.machine, s'.machine)
+    && s'.disk == s.disk
+  }
+
+  predicate NextStep(k: Constants, s: Variables, s': Variables, step: Step)
+  {
+    match step {
+      case MachineStep(dop) => Machine(k, s, s', dop)
+      case CrashStep => Crash(k, s, s')
+    }
+  }
+
+  predicate Next(k: Constants, s: Variables, s': Variables) {
+    exists step :: NextStep(k, s, s', step)
+  }
+
+  // Invariant
+
+  predicate Inv(k: Constants, s: Variables) {
+    && BCS.Inv(k, s)
+    // TODO add btree invariants here
+  }
+
+  // Proofs
+
+  lemma InitImpliesInv(k: Constants, s: Variables)
+    requires Init(k, s)
+    ensures Inv(k, s)
+  {
+    BCS.InitImpliesInv(k, s);
+  }
+
+  lemma BetreeMoveStepPreservesInv(k: Constants, s: Variables, s': Variables, dop: DiskOp, step: DB.Step)
+    requires Inv(k, s)
+    requires M.BetreeMove(k.machine, s.machine, s'.machine, dop, step)
+    requires s.disk == s'.disk
+    ensures Inv(k, s')
+
+  lemma BlockCacheStepPreservesInv(k: Constants, s: Variables, s': Variables, dop: DiskOp, step: BC.Step)
+    requires Inv(k, s)
+    requires M.BlockCacheMove(k.machine, s.machine, s'.machine, dop, step)
+    requires Machine(k, s, s', dop)
+    ensures Inv(k, s')
+  {
+    assert BCS.Machine(k, s, s', dop);
+    assert BCS.NextStep(k, s, s', BCS.MachineStep(dop));
+    BCS.NextPreservesInv(k, s, s');
+  }
+
+  lemma MachineStepPreservesInv(k: Constants, s: Variables, s': Variables, dop: DiskOp)
+    requires Inv(k, s)
+    requires Machine(k, s, s', dop)
+    ensures Inv(k, s')
+  {
+    var step :| M.NextStep(k.machine, s.machine, s'.machine, dop, step);
+    match step {
+      case BetreeMoveStep(betreeStep) => BetreeMoveStepPreservesInv(k, s, s', dop, betreeStep);
+      case BlockCacheMoveStep(blockCacheStep) => BlockCacheStepPreservesInv(k, s, s',dop, blockCacheStep);
+    }
+  }
+
+  lemma CrashStepPreservesInv(k: Constants, s: Variables, s': Variables)
+    requires Inv(k, s)
+    requires Crash(k, s, s')
+    ensures Inv(k, s')
+  {
+    
+  }
+
+  lemma NextStepPreservesInv(k: Constants, s: Variables, s': Variables, step: Step)
+    requires Inv(k, s)
+    requires NextStep(k, s, s', step)
+    ensures Inv(k, s')
+  {
+    match step {
+      case MachineStep(dop: DiskOp) => MachineStepPreservesInv(k, s, s', dop);
+      case CrashStep => CrashStepPreservesInv(k, s, s');
+    }
+  }
+
+  lemma NextPreservesInv(k: Constants, s: Variables, s': Variables)
+    requires Inv(k, s)
+    requires Next(k, s, s')
+    ensures Inv(k, s')
+  {
+    var step :| NextStep(k, s, s', step);
+    NextStepPreservesInv(k, s, s', step);
+  }
+}
